definitions + first proofs

operations/Linearize2.thy
@@ -160,8 +160,6 @@ mrbnf "('a, 'b :: var, 'c :: var, 'd, 'e :: var, 'f) F"
   var_class: var
   sorry
 
-ML \<open>MRBNF_Def.mrbnf_of @{context} @{type_name F} |> the |> MRBNF_Def.var_types_of_mrbnf\<close>
-
 typedef 'a foo = "{x::'a \<times> 'a list. snd x = []}"
   by simp
 
@@ -170,11 +168,20 @@ lift_bnf_2 (no_warn_wits, no_warn_transfer) 'a foo
 (*
 binder_datatype ('a, 'b::var) test = V 'b | B "'a set" | C x::'b t::"('a, 'b) test" binds x in t
 *)
-linearize_mrbnf ('a, F'bset: 'b :: var, 'c :: var, 'd, 'e :: var, 'f) F' = "('a, 'b, 'c, 'd, 'e, 'f) F" on 'a
+
+(*declare [[quick_and_dirty]]*)
+
+
+linearize_mrbnf ('a, F''bset: 'b :: var, 'c :: var, 'd, 'e :: var, 'f) F'' = "('a, 'b, 'c, 'd, 'e, 'f) F" on 'a
   sorry
 
-thm mr_rel_F_def
+thm sameShape_F_def nonrep_F_def
+thm asSS_F''_def (* should this just be globally defined somewhere? it's not connected to F or F'' *)
 
+thm F.map_id
+find_theorems name: F.map
+find_theorems name: F''.map (* where are the mrbnf theorems? *)
+find_theorems name: map_comp0
 
 (* we linearize this MRBNF on position 1*)
 ML \<open>val lin_pos = 1\<close>
@@ -192,8 +199,6 @@ axiomatization where
   (* The next property assumes that nonrepetitive elements exist: *)
   ex_nonrep: "\<exists>x. \<forall>x'. (\<exists> R. rrel_F R (=) x x') \<longrightarrow> (\<exists> f. x' = map_F f id id id id x)"
 
-abbreviation "rel_F \<equiv> mr_rel_F"
-
 (* Important consequence of preservation of pullbacks (which is actually equivalent to it): 
 The relator is closed under intersections. *)
 
@@ -206,8 +211,9 @@ fun mk_F_strong_tac mrbnf F_map_id mr_rel_F_def F_mr_rel_mono_strong0 F_rel_map_
     val var_types = var_types_of_mrbnf mrbnf;
     val nr_lives = length (filter (fn v => v = MRBNF_Def.Live_Var) var_types);
   in
+    print_tac ctxt "Start" THEN
     HEADGOAL (
-      forward_tac ctxt [F_mr_rel_mono_strong0 OF flat (replicate 2 id_prems)] THEN_ALL_NEW (
+      forward_tac ctxt ([F_mr_rel_mono_strong0 OF flat (replicate 2 id_prems)] |> @{print}) THEN_ALL_NEW (
         TRY o (rtac ctxt ballI THEN_ALL_NEW 
           resolve_tac ctxt [ballI, refl]) THEN_ALL_NEW
         TRY o (rtac ctxt impI THEN_ALL_NEW
@@ -254,7 +260,8 @@ fun mk_F_strong_tac mrbnf F_map_id mr_rel_F_def F_mr_rel_mono_strong0 F_rel_map_
 \<close>
 
 lemma F_strong:
-  "rel_F R1 id id R4 id x y \<Longrightarrow> rel_F Q1 id id Q4 id x y \<Longrightarrow> rel_F  (inf R1 Q1) id id (inf R4 Q4) id x y"
+  "mr_rel_F R1 id id R4 id x y \<Longrightarrow> mr_rel_F Q1 id id Q4 id x y \<Longrightarrow> mr_rel_F  (inf R1 Q1) id id (inf R4 Q4) id x y"
+  apply -
   by (tactic \<open>mk_F_strong_tac (MRBNF_Def.mrbnf_of @{context} @{type_name F} |> the) @{thm F.map_id} @{thm mr_rel_F_def} @{thm F.mr_rel_mono_strong0}
     @{thm F_rel_map_set2_strong} @{thm F.in_rel} @{context} 
     THEN print_tac @{context} "done"\<close>)
@@ -288,8 +295,8 @@ fun mk_rel_F_exchange_tac mrbnf F_mr_rel_mono_strong0 F_strong ctxt =
 Since the atoms have a fixed position, we can permute the relations: *)
 lemma rel_F_exchange: 
   fixes x :: "('a, 'b :: var, 'c :: var, 'd, 'e :: var, 'f) F" and x' :: "('a', 'b, 'c, 'd', 'e, 'f) F"
-  assumes "rel_F R1 id id R4 id x x'" and "rel_F Q1 id id Q4 id x x'"
-  shows "rel_F R1 id id Q4 id x x'" 
+  assumes "mr_rel_F R1 id id R4 id x x'" and "mr_rel_F Q1 id id Q4 id x x'"
+  shows "mr_rel_F R1 id id Q4 id x x'" 
   using assms apply -
   by (tactic \<open>mk_rel_F_exchange_tac (MRBNF_Def.mrbnf_of @{context} @{type_name F} |> the) 
     @{thm F.mr_rel_mono_strong0} @{thm F_strong} @{context} 
@@ -298,7 +305,7 @@ lemma rel_F_exchange:
 (* Then notion of two items having the same shape (w.r.t. the 1st position): *)
 (* these definitions are lin_pos dependent *)
 definition sameShape1 :: "('a1,'a2::var,'a3::var,'a4,'a5::var,'a6) F \<Rightarrow> ('a1,'a2,'a3,'a4,'a5,'a6) F \<Rightarrow> bool" where 
-  "sameShape1 x x' \<equiv> \<exists> R. rel_F R id id (=) id x x'"
+  "sameShape1 x x' \<equiv> \<exists> R. mr_rel_F R id id (=) id x x'"
 
 definition nonrep2 :: "('a1,'a2::var,'a3::var,'a4,'a5::var,'a6) F \<Rightarrow> bool" where 
   "nonrep2 x \<equiv> \<forall> x'. sameShape1 x x' \<longrightarrow> (\<exists> f. x' = map_F f id id id id x)"
@@ -329,16 +336,16 @@ fun mk_nonrep2_map_F_tac mrbnf nonrep_def sameShape_def F_map_comp F_mr_rel_map 
           etac ctxt exE,
           EqSubst.eqsubst_tac ctxt [0] [F_map_comp] THEN_ALL_NEW
             TRY o resolve_tac ctxt (prems @ @{thms supp_id_bound bij_id}),
-          K (unfold_tac ctxt [switch id_o o_id]),
+          K (unfold_thms_tac ctxt [switch id_o o_id]),
           EqSubst.eqsubst_tac ctxt [lin_pos] [switch o_id id_o], (*move all id to the right except for lin_pos*)
           EqSubst.eqsubst_tac ctxt [0] [F_map_comp RS sym] THEN_ALL_NEW
             TRY o resolve_tac ctxt (prems @ @{thms supp_id_bound bij_id}),
           dtac ctxt (rotate_prems ~1 (F_mr_rel_map RS iffD1)) THEN_ALL_NEW
             TRY o resolve_tac ctxt (prems @ @{thms supp_id_bound bij_id}),
-          K (unfold_tac ctxt [switch id_o o_id, @{thm Grp_UNIV_id}]),
-          K (unfold_tac ctxt [switch @{thm OO_eq} @{thm eq_OO}]),  
+          K (unfold_thms_tac ctxt [switch id_o o_id, @{thm Grp_UNIV_id}]),
+          K (unfold_thms_tac ctxt [switch @{thm OO_eq} @{thm eq_OO}]),  
           EqSubst.eqsubst_asm_tac ctxt [lin_live_pos] [switch @{thm eq_OO} @{thm OO_eq}], (*move all (=) to the left except for lin_live_pos*)
-          K (unfold_tac ctxt @{thms eq_alt}),   
+          K (unfold_thms_tac ctxt @{thms eq_alt}),   
           EqSubst.eqsubst_tac ctxt [0] @{thms Grp_UNIV_id}
         ]) THEN
         unfold_thms_tac ctxt [mr_rel_F_def, o_id, F_rel_compp, F_rel_Grp, F_map_id] THEN
@@ -429,7 +436,7 @@ fun mk_nonrep2_map_F_rev_tac mrbnf nonrep_def sameShape_def F_mr_rel_map1 F_mr_r
           rotate_tac 1,
           EqSubst.eqsubst_asm_tac ctxt (map_range (fn i => i+1) nr_non_lives) [switch @{thm o_id} @{thm id_o}],
           EqSubst.eqsubst_asm_tac ctxt [lin_live_pos] @{thms Grp_UNIV_id},
-          K (unfold_tac ctxt [switch @{thm eq_OO} @{thm OO_eq}]),
+          K (unfold_thms_tac ctxt [switch @{thm eq_OO} @{thm OO_eq}]),
           EqSubst.eqsubst_asm_tac ctxt [lin_live_pos] [switch @{thm OO_eq} @{thm eq_OO}], (*move all (=) to the right and then lin_live_pos back*)
           EqSubst.eqsubst_asm_tac ctxt [lin_live_pos] @{thms eq_alt},
           EqSubst.eqsubst_asm_tac ctxt [0] [F_mr_rel_map1 RS sym] THEN_ALL_NEW
@@ -443,16 +450,16 @@ fun mk_nonrep2_map_F_rev_tac mrbnf nonrep_def sameShape_def F_mr_rel_map1 F_mr_r
           etac ctxt exE,
           EqSubst.eqsubst_asm_tac ctxt [0] [F_map_comp] THEN_ALL_NEW
             TRY o resolve_tac ctxt (prems @ @{thms supp_id_bound bij_id}),
-          K (unfold_tac ctxt @{thms id_o o_id}),
+          K (unfold_thms_tac ctxt @{thms id_o o_id}),
           EqSubst.eqsubst_asm_tac ctxt [1] [F_rel_eq RS sym],
           EqSubst.eqsubst_asm_tac ctxt [1] [F_mr_rel_id],
           dtac ctxt (rotate_prems ~1 (iffD1 OF [F_mr_rel_map1])) THEN_ALL_NEW
             TRY o resolve_tac ctxt (prems @ @{thms supp_id_bound bij_id}),
-          K (unfold_tac ctxt @{thms id_o OO_eq}),
+          K (unfold_thms_tac ctxt @{thms id_o OO_eq}),
           dtac ctxt (rotate_prems 1 rel_F_exchange),
           rtac ctxt (F_mr_rel_flip RS iffD1) THEN_ALL_NEW
             TRY o resolve_tac ctxt @{thms supp_id_bound bij_id},
-          K (unfold_tac ctxt @{thms inv_id}),
+          K (unfold_thms_tac ctxt @{thms inv_id}),
           EqSubst.eqsubst_asm_tac ctxt [0] [F_mr_rel_map3] THEN_ALL_NEW
             TRY o resolve_tac ctxt (prems @ @{thms supp_id_bound bij_id}),
           EqSubst.eqsubst_asm_tac ctxt (map_range (fn i => i+1) (2 * nr_lives)) @{thms Grp_def},
@@ -522,23 +529,23 @@ fun mk_nonrep2_map_bij_tac mrbnf nonrep_def sameShape_def F_mr_rel_map1 F_mr_rel
           if (v = MRBNF_Def.Live_Var andalso i+1 < lin_pos) then b+1 else b) var_types 1;
         val o_id_poses = map_range (fn i => if i < lin_pos-1 then i*2 + 7 else (i+1)*2 + 7) (length var_types-1) |> filter (fn n => n >= 0);
       in
-        unfold_tac ctxt [nonrep_def, sameShape_def] THEN
+        unfold_thms_tac ctxt [nonrep_def, sameShape_def] THEN
         HEADGOAL (EVERY' [
           rtac ctxt allI,
           rtac ctxt impI,
           etac ctxt exE,
           dtac ctxt (rotate_prems ~1 (F_mr_rel_map1 RS iffD1)) THEN_ALL_NEW
             TRY o resolve_tac ctxt @{thms bij_id supp_id_bound},
-          K (unfold_tac ctxt @{thms o_id Grp_UNIV_id}),
+          K (unfold_thms_tac ctxt @{thms o_id Grp_UNIV_id}),
           EqSubst.eqsubst_asm_tac ctxt [lin_live_pos*3 - 1] [@{thm OO_eq} RS sym],
           EqSubst.eqsubst_asm_tac ctxt (map_range (fn i => i+1) (nr_lives*2 -1)) [@{thm conversep_eq} RS sym],
           EqSubst.eqsubst_asm_tac ctxt (map_range (fn i => i+1) (nr_lives*2 -1)) @{thms eq_alt},
           EqSubst.eqsubst_asm_tac ctxt [1] [@{thm inv_o_simp2} OF [(nth prems 0)] RS sym],
-          K (unfold_tac ctxt @{thms Grp_o converse_relcompp}),
+          K (unfold_thms_tac ctxt @{thms Grp_o converse_relcompp}),
           EqSubst.eqsubst_asm_tac ctxt [1] [@{thm relcompp_assoc} RS sym],
           dtac ctxt ((unfold_thms ctxt @{thms inv_id o_id} (F_mr_rel_map3 OF 
             (id_prems @ id_prems_v) RS sym)) RS iffD1),
-          K (unfold_tac ctxt @{thms Grp_UNIV_id conversep_eq}),
+          K (unfold_thms_tac ctxt @{thms Grp_UNIV_id conversep_eq}),
           dtac ctxt (Object_Logic.rulify ctxt (unfold_thms ctxt [nonrep_def, sameShape_def] (nth prems 1)) OF [exI]),
           etac ctxt exE
         ]) THEN
@@ -548,11 +555,11 @@ fun mk_nonrep2_map_bij_tac mrbnf nonrep_def sameShape_def F_mr_rel_map1 F_mr_rel
               EqSubst.eqsubst_tac ctxt [0] [F_map_id RS sym],
               EqSubst.eqsubst_tac ctxt o_id_poses [@{thm o_id} RS sym],
               EqSubst.eqsubst_tac ctxt [1] [@{thm inv_o_simp2} OF [(nth prems 0)] RS sym],
-              K (unfold_tac ctxt [F_map_comp OF flat (replicate 2 id_prems) RS sym]),
+              K (unfold_thms_tac ctxt [F_map_comp OF flat (replicate 2 id_prems) RS sym]),
               EqSubst.eqsubst_tac ctxt [1] subprems,
               EqSubst.eqsubst_tac ctxt [2*lin_pos + 6 + 2*(length var_types)] [@{thm o_id} RS sym],
               EqSubst.eqsubst_tac ctxt [1] [@{thm inv_o_simp1} OF [(nth prems 0)] RS sym],
-              K (unfold_tac ctxt [F_map_comp OF flat (replicate 2 id_prems)]),
+              K (unfold_thms_tac ctxt [F_map_comp OF flat (replicate 2 id_prems)]),
               EqSubst.eqsubst_tac ctxt [1, 2] @{thms o_assoc},
               rtac ctxt exI,
               rtac ctxt refl
@@ -601,8 +608,7 @@ lemma nonrep2_mapF_bij_2:
 
 
 typedef ('a1,'a2::var,'a3::var,'a4,'a5::var,'a6) F' = "{x :: ('a1,'a2,'a3,'a4,'a5,'a6) F. nonrep2 x}"
-  apply (unfold mem_Collect_eq nonrep2_def sameShape1_def mr_rel_F_def F.map_id id_apply)
-  apply (unfold id_def[symmetric])
+  apply (unfold mem_Collect_eq nonrep2_def sameShape1_def mr_rel_F_def F.map_id)
   by (rule ex_nonrep)
 
 definition set1_F' :: "('a1,'a2::var,'a3::var,'a4,'a5::var,'a6) F' \<Rightarrow> 'a1 set" where "set1_F' = set1_F o Rep_F'"
@@ -654,13 +660,13 @@ fun mk_map_comp_tac mrbnf map_F'_def Abs_F'_inverse Rep_F' nonrep2_mapF_bij_2 F_
       val nr_bounds = length (filter (fn v => v = MRBNF_Def.Bound_Var) var_types);
       val nr_frees = length (filter (fn v => v = MRBNF_Def.Free_Var) var_types);
     in
-      unfold_tac ctxt (map_F'_def:: @{thms asSS_def asBij_def}) THEN
+      unfold_thms_tac ctxt (map_F'_def:: @{thms asSS_def asBij_def}) THEN
       HEADGOAL(EqSubst.eqsubst_tac ctxt (map_range (fn i => i+1) (1 + 2*nr_bounds)) @{thms bij_comp} THEN_ALL_NEW
         TRY o resolve_tac ctxt prems) THEN
-      unfold_tac ctxt @{thms if_True} THEN
+      unfold_thms_tac ctxt @{thms if_True} THEN
       HEADGOAL (EqSubst.eqsubst_tac ctxt (map_range (fn i => i+1) (nr_bounds + nr_frees)) @{thms supp_comp_bound} THEN_ALL_NEW
         TRY o resolve_tac ctxt (@{thm infinite_UNIV} ::prems)) THEN
-      unfold_tac ctxt (@{thm if_True} :: map (fn thm => thm RS eqTrueI) prems) THEN
+      unfold_thms_tac ctxt (@{thm if_True} :: map (fn thm => thm RS eqTrueI) prems) THEN
       HEADGOAL (rtac ctxt ext) THEN
       HEADGOAL (EqSubst.eqsubst_tac ctxt [1] [F_map_comp0] THEN_ALL_NEW
         TRY o resolve_tac ctxt prems) THEN
@@ -841,14 +847,16 @@ fun mk_rel_comp_leq_tac rrel_F'_def F_rel_compp ctxt =
   HEADGOAL (EVERY' [
     rtac ctxt @{thm predicate2I},
     etac ctxt @{thm relcomppE},
-    K (unfold_tac ctxt [rrel_F'_def]),
+    K (unfold_thms_tac ctxt [rrel_F'_def]),
+    K (print_tac ctxt "state1"),
     EqSubst.eqsubst_tac ctxt [1] (@{thms eq_OO[symmetric]}),
+    K (print_tac ctxt "state2"),
     EqSubst.eqsubst_tac ctxt [1] ([F_rel_compp]),
-    K (unfold_tac ctxt [rrel_F'_def]),
+    K (unfold_thms_tac ctxt [rrel_F'_def]),
     rtac ctxt @{thm relcomppI} THEN_ALL_NEW assume_tac ctxt
   ])
 \<close>
-
+thm F.rel_compp F.map_id
 lemma F'_rel_comp_leq_: "rrel_F' Q OO rrel_F' R \<le> rrel_F' (Q OO R)"
   by (tactic \<open>mk_rel_comp_leq_tac @{thm rrel_F'_def} @{thm F.rel_compp} @{context}
     THEN print_tac @{context} "done"\<close>)
@@ -984,7 +992,7 @@ fun mk_in_rel_tac mrbnf rrel_F'_def map_F'_def Abs_F'_inverse Rep_F' nonrep2_map
             REPEAT_DETERM_N (nr_lives) (
               HEADGOAL (EqSubst.eqsubst_tac ctxt [0] F_set_maps THEN_ALL_NEW
                 TRY o resolve_tac ctxt @{thms bij_id supp_id_bound})) THEN
-            unfold_tac ctxt @{thms image_ident} THEN
+            unfold_thms_tac ctxt @{thms image_ident} THEN
             REPEAT_DETERM_N (nr_lives-1) (
               HEADGOAL (rtac ctxt conjI THEN_ALL_NEW
                 TRY o resolve_tac ctxt subprems)) THEN
